Fix Coq 8.14 by renaming files

theories/Iris/Model.v
@@ -28,1477 +28,283 @@
 
 From Equations Require Import
      Equations Signature.
-Require Import Equations.Prop.EqDec.
-
-From stdpp Require finite gmap list.
 
 From iris Require Import
      algebra.auth
      algebra.excl
      algebra.gmap
-     base_logic.lib.fancy_updates
-     base_logic.lib.gen_heap
-     base_logic.lib.own
-     bi.big_op
-     bi.interface
      program_logic.adequacy
      program_logic.weakestpre
      proofmode.tactics.
 
 From Katamaran Require Import
-     Iris.Base
-     SmallStep.Step
-     SmallStep.Inversion
+     Prelude
      Sep.Logic
-     Sep.Hoare
-     Signature
-     Specification
-     Semantics
-     Prelude.
-
-Import ctx.notations.
-Import env.notations.
+     Semantics.
 
 Set Implicit Arguments.
 
-Module Type IrisPredicates
+Section TransparentObligations.
+  Local Set Transparent Obligations.
+  (* Derive NoConfusion for SomeReg. *)
+  (* Derive NoConfusion for SomeVal. *)
+  Derive NoConfusion for iris.algebra.excl.excl.
+End TransparentObligations.
+
+Program Definition IProp Σ : SepLogic :=
+  {| lcar              := iProp Σ;
+     lentails          := bi_entails;
+     sep.land          := bi_and;
+     sep.lor           := bi_or;
+     limpl             := bi_impl;
+     lprop             := bi_pure;
+     lex               := @bi_exist _;
+     lall              := @bi_forall _;
+     lemp              := bi_emp;
+     lsep              := bi_sep;
+     lwand             := bi_wand;
+     lentails_preorder := bi.entails_po;
+     land_right        := bi.and_intro;
+     land_left1        := bi.and_elim_l';
+     land_left2        := bi.and_elim_r';
+     lor_left          := bi.or_elim;
+     lor_right1        := bi.or_intro_l';
+     lor_right2        := bi.or_intro_r';
+     lex_right         := fun B x P Q => @bi.exist_intro' _ B P Q x;
+     lex_left          := @bi.exist_elim _;
+     lall_left         := fun B x P Q => transitivity (bi.forall_elim x);
+     lall_right        := fun B => bi.forall_intro;
+     limpl_and_adjoint := fun P Q R => conj (bi.impl_intro_r P Q R) (bi.impl_elim_l' P Q R);
+     lprop_left        := bi.pure_elim';
+     lprop_right       := bi.pure_intro;
+     lsep_assoc        := fun P Q R => proj1 (bi.equiv_entails _ _) (bi.sep_assoc P Q R);
+     lsep_comm         := fun P Q => proj1 (bi.equiv_entails _ _) (bi.sep_comm P Q);
+     lwand_sep_adjoint := fun P Q R => conj (bi.wand_intro_r P Q R) (bi.wand_elim_l' P Q R);
+     lsep_andp_prop    := _;
+     lsep_entails      := fun P P' Q Q' => bi.sep_mono P Q P' Q';
+     lsep_emp          := fun P => proj1 (bi.equiv_entails _ _) (bi.sep_emp P);
+     lsep_leak         := _;
+  |}.
+Next Obligation.
+  intros Σ P R Q. split.
+  - iIntros "[P [% R]]".
+    by iSplit; iFrame.
+  - iIntros "[% [P R]]".
+    by iFrame.
+Qed.
+Next Obligation.
+  now iIntros (Σ P) "HP".
+Qed.
+Canonical IProp.
+
+Module Type IrisPrelims
+    (Import B    : Base)
+    (Import PROG : Program B)
+    (Import SEM  : Semantics B PROG).
+
+  Import SmallStepNotations.
+
+  Section Language.
+
+    (* The "expressions" of the LanguageMixin are configurations consisting of a
+       statement and a local variable store. *)
+    Record Conf (Γ : PCtx) τ : Type :=
+      MkConf
+        { conf_stm   : Stm Γ τ;
+          conf_store : CStore Γ
+        }.
+
+    Section TransparentObligations.
+      Local Set Transparent Obligations.
+      Derive NoConfusion for Conf.
+    End TransparentObligations.
+
+    (* The "values" of the LanguageMixin are final configurations consisting of a
+       value and a store. We only keep the store around for technical reasons,
+       essentially to validate of_to_val. *)
+    Section ValConf.
+      Local Set Primitive Projections.
+      Record ValConf (Γ : PCtx) τ : Type :=
+        MkValConf
+          { valconf_val   : Val τ;
+            valconf_store : CStore Γ
+          }.
+    End ValConf.
+
+    Definition of_val {Γ} {τ} (v : ValConf Γ τ) : Conf Γ τ :=
+      match v with
+        MkValConf _ v δ => MkConf (stm_val _ v) δ
+      end.
+
+    Definition to_val {Γ} {τ} (t : Conf Γ τ) : option (ValConf Γ τ) :=
+      match t with
+      | MkConf (stm_val _ v) δ => Some (MkValConf _ v δ)
+      | _                      => None
+      end.
+
+    Lemma to_of_val {Γ} {τ} (v : ValConf Γ τ) : to_val (of_val v) = Some v.
+    Proof.
+      by destruct v.
+    Qed.
+
+    Lemma of_to_val {Γ} {τ} (s : Conf Γ τ) v : to_val s = Some v → of_val v = s.
+    Proof.
+      destruct s as [s δ]; destruct s; try done.
+      by intros [= <-].
+    Qed.
+
+    Lemma val_head_stuck_step {τ} {Γ : PCtx} γ1 γ2 μ1 μ2 (δ1 : CStore Γ) δ2 (s1 : Stm Γ τ) s2 :
+      ⟨ γ1, μ1, δ1, s1 ⟩ ---> ⟨ γ2, μ2, δ2, s2 ⟩ -> to_val (MkConf s1 δ1) = None.
+    Proof.
+      by induction 1.
+    Qed.
+
+    Definition observation := Empty_set.
+
+    Definition State := prod RegStore Memory.
+
+    Inductive prim_step {Γ τ} : Conf Γ τ -> State -> list Empty_set -> Conf Γ τ -> State -> list (Conf Γ τ) -> Prop :=
+    | mk_prim_step γ1 γ2 μ1 μ2 (δ1 : CStore Γ) (δ2 : CStore Γ) s1 s2 :
+        ⟨ γ1, μ1, δ1, s1 ⟩ ---> ⟨ γ2, μ2, δ2, s2 ⟩ ->
+        prim_step (MkConf s1 δ1) (γ1 , μ1) nil (MkConf s2 δ2) (γ2 , μ2) nil
+    .
+
+    Lemma val_head_stuck {Γ τ} (e1 : Conf Γ τ) s1 ls e2 s2 {ks} : prim_step e1 s1 ls e2 s2 ks → to_val e1 = None.
+    Proof.
+      induction 1.
+      by eapply val_head_stuck_step.
+    Qed.
+
+    Lemma microsail_lang_mixin Γ τ : LanguageMixin of_val to_val (@prim_step Γ τ).
+    Proof. split; eauto using to_of_val, of_to_val, val_head_stuck. Qed.
+
+    Canonical Structure microsail_lang Γ τ : language := Language (microsail_lang_mixin Γ τ).
+
+    #[export] Instance intoVal_valconf {Γ τ δ v} : IntoVal (MkConf (Γ := Γ) (τ := τ) (stm_val _ v) δ) (MkValConf _ v δ).
+      intros; eapply of_to_val; by cbn.
+    Defined.
+
+  End Language.
+
+  Section Registers.
+
+    Definition SomeReg : Type := sigT 𝑹𝑬𝑮.
+    Definition SomeVal : Type := sigT Val.
+
+    #[export] Instance eqDec_SomeReg : EqDec SomeReg := 𝑹𝑬𝑮_eq_dec.
+    #[export] Instance countable_SomeReg : countable.Countable SomeReg := finite.finite_countable.
+
+    #[export] Instance eqDec_SomeVal : EqDec SomeVal.
+    Proof.
+      intros [τ1 v1] [τ2 v2].
+      destruct (eq_dec τ1 τ2).
+      - subst.
+        destruct (Val_eqb_spec _ v1 v2).
+        + left. congruence.
+        + right. intros H.
+          Local Set Equations With UIP.
+          by dependent elimination H.
+      - right. intros H.
+        by dependent elimination H.
+    Qed.
+
+    Definition regUR := authR (gmapUR SomeReg (exclR (leibnizO SomeVal))).
+    (* Definition regUR' : cmra := *)
+    (*   authR (discrete_funUR (A := SomeReg) *)
+    (*            (fun '(existT σ r) => excl_auth.excl_authUR (leibnizO (Val σ)))). *)
+
+    Class sailRegGS Σ := SailRegGS {
+                            (* ghost variable for tracking state of registers *)
+                            reg_inG : inG Σ regUR;
+                            reg_gv_name : gname;
+                          }.
+    #[export] Existing Instance reg_inG.
+
+    Definition reg_pointsTo `{sailRegGS Σ} {τ} (r : 𝑹𝑬𝑮 τ) (v : Val τ) : iProp Σ :=
+      own reg_gv_name (◯ {[ existT _ r := Excl (existT _ v) ]}).
+
+    Definition regs_inv `{sailRegGS Σ} (regstore : RegStore) : iProp Σ :=
+      (∃ regsmap,
+          own reg_gv_name (● regsmap) ∗
+          ⌜ map_Forall (K := SomeReg) (A := excl SomeVal) (fun reg v => match reg with | existT _ reg => Excl (existT _ (read_register regstore reg)) = v end ) regsmap ⌝
+      )%I.
+
+  End Registers.
+End IrisPrelims.
+
+Module Type IrisParameters
   (Import B    : Base)
   (Import PROG : Program B)
   (Import SEM  : Semantics B PROG)
-  (Import SIG  : Signature B)
-  (Import IB   : IrisBase B PROG SEM).
-  Parameter luser_inst : forall `{sRG : sailRegGS Σ} `{invGS Σ} (mG : memGS Σ) (p : 𝑯) (ts : Env Val (𝑯_Ty p)), iProp Σ.
-  Parameter lduplicate_inst : forall `{sRG : sailRegGS Σ} `{invGS Σ} (mG : memGS Σ) (p : 𝑯) (ts : Env Val (𝑯_Ty p)),
-      is_duplicable p = true -> bi_entails (luser_inst (sRG := sRG) mG ts) (luser_inst (sRG := sRG) mG ts ∗ luser_inst (sRG := sRG) mG ts).
-
-End IrisPredicates.
-
-(*
- * The following module defines the Iris model depending solely on the Signature, not only the Specification.
- * This allows us to use multiple different specifications with the same Iris model, so that the resulting triples can be combined.
- * This is important particularly in the RiscvPmp.BlockVerification proofs.
- *)
-Module Type IrisSignatureRules
-  (Import B     : Base)
-  (Import PROG  : Program B)
-  (Import SEM   : Semantics B PROG)
-  (Import SIG   : Signature B)
-  (Import IB    : IrisBase B PROG SEM)
-  (Import IPred : IrisPredicates B PROG SEM SIG IB).
-Section Soundness.
-
-  Import SmallStepNotations.
-
-  Context `{sG : sailGS Σ}.
-
-  #[export] Instance PredicateDefIProp : PredicateDef (IProp Σ) :=
-    {| lptsreg σ r v        := reg_pointsTo r v;
-       luser p ts           := luser_inst sailGS_memGS ts;
-       lduplicate p ts Hdup := lduplicate_inst (sRG := sailGS_sailRegGS) sailGS_memGS ts Hdup
-    |}.
-
-  Lemma reg_valid regstore {τ} (r : 𝑹𝑬𝑮 τ) (v : Val τ) :
-    ⊢ (regs_inv regstore -∗ reg_pointsTo r v -∗ ⌜read_register regstore r = v⌝)%I.
-  Proof.
-    iDestruct 1 as (regsmap) "[Hregs %]".
-    iIntros "Hreg".
-    iDestruct (own_valid_2 with "Hregs Hreg") as %[Hl regsv]%auth_both_valid.
-    iPureIntro.
-    specialize (Hl 0).
-    setoid_rewrite (singleton_includedN_l 0 regsmap (existT _ r) _) in Hl.
-    destruct Hl as [y [eq1%discrete%leibniz_equiv eq2%cmra_discrete_included_r]];
-      auto with typeclass_instances.
-    specialize (regsv (existT _ r)).
-    rewrite eq1 in regsv.
-    destruct y as [y|]; [|inversion regsv].
-    setoid_rewrite Excl_included in eq2.
-    apply leibniz_equiv in eq2. subst.
-    specialize (H (existT _ r) (Excl (existT _ v)) eq1); cbn in H.
-    Local Set Equations With UIP.
-    by dependent elimination H.
-  Qed.
-
-  Lemma regs_inv_update {τ} {r} {v : Val τ} {regsmap : gmapUR SomeReg (exclR (leibnizO SomeVal))} {regstore : RegStore} :
-    map_Forall (K := SomeReg) (A := excl SomeVal) (λ r' v', match r' with
-                         | existT τ r'' => Excl (existT _ (read_register regstore r'')) = v'
-                         end) regsmap ->
-    (own reg_gv_name (● <[existT _ r:=Excl (existT _ v)]> regsmap)) -∗ regs_inv (write_register regstore r v).
-  Proof.
-    iIntros (regseq) "Hownregs".
-    iExists (<[existT _ r:=Excl (existT _ v)]> regsmap).
-    iFrame.
-    iPureIntro.
-    apply (map_Forall_lookup_2 _ (<[existT _ r:=Excl (existT _ v)]> regsmap)).
-    intros [τ' r'] x eq1.
-    destruct (eq_dec_het r r') as [eq2|neq].
-    + dependent elimination eq2.
-      rewrite lookup_insert in eq1.
-      apply (inj Some) in eq1.
-      by rewrite <- eq1, (read_write regstore r v).
-    + assert (existT _ r ≠ existT _ r') as neq2.
-      * intros eq2.
-        dependent elimination eq2.
-        now apply neq.
-      * rewrite (lookup_insert_ne _ _ _ _ neq2) in eq1.
-        rewrite (read_write_distinct _ _ neq).
-        apply (map_Forall_lookup_1 _ _ _ _ regseq eq1).
-  Qed.
-
-  Lemma reg_update regstore {τ} r (v1 v2 : Val τ) :
-    regs_inv regstore -∗ reg_pointsTo r v1 ==∗ regs_inv (write_register regstore r v2) ∗ reg_pointsTo r v2.
-  Proof.
-    iDestruct 1 as (regsmap) "[Hregs %]".
-    rewrite /reg_pointsTo.
-    iIntros "Hreg".
-    iDestruct (own_valid_2 with "Hregs Hreg") as %[Hl%cmra_discrete_included_r regsmapv]%auth_both_valid.
-    setoid_rewrite (singleton_included_l regsmap (existT _ r) _) in Hl.
-    destruct Hl as [y [eq1%leibniz_equiv eq2]].
-    specialize (regsmapv (existT _ r)).
-    rewrite eq1 in regsmapv.
-    destruct y as [y|]; inversion regsmapv.
-    iMod (own_update_2 with "Hregs Hreg") as "[Hregs Hreg]".
-    {
-      eapply auth_update.
-      apply (singleton_local_update regsmap (existT _ r) (Excl y) (Excl (existT _ v1)) (Excl (existT _ v2)) (Excl (existT _ v2)) eq1).
-      by eapply exclusive_local_update.
-    }
-    iModIntro.
-    iFrame.
-    iApply (regs_inv_update H); iFrame.
-  Qed.
-
-  Definition semTriple {Γ τ} (δ : CStore Γ)
-             (PRE : iProp Σ) (s : Stm Γ τ) (POST : Val τ -> CStore Γ -> iProp Σ) : iProp Σ :=
-    PRE -∗ WP (MkConf s δ : expr (microsail_lang Γ τ)) ?{{ v, POST (valconf_val v) (valconf_store v) }}.
-  (* always modality needed? perhaps not because sail not higher-order? *)
-
-  Lemma wp_compat_fail {Γ τ} {s} {δ} {Q : ValConf Γ τ -> iProp Σ} :
-    (⊢ WP (MkConf (stm_fail _ s) δ) ?{{ v, Q v }})%I.
-  Proof.
-    rewrite wp_unfold. cbn.
-    iIntros (σ _ ks1 ks nt) "Hregs".
-    iMod (fupd_mask_subseteq empty) as "Hclose"; first set_solver.
-    iModIntro.
-    iSplitR; [trivial|].
-    iIntros (e2 σ2 efs) "%".
-    remember (MkConf (fail s) δ) as s1.
-    destruct H.
-    inversion Heqs1. subst.
-    inversion H.
-  Qed.
-
-  Lemma wp_compat_block {Γ Δ} {τ : Ty} {δ : CStore Γ}
-        (δΔ : CStore Δ) (k : Stm (Γ ▻▻ Δ) τ) (Q : ValConf Γ τ -> iProp Σ) :
-    ⊢ (WP (MkConf k (δ ►► δΔ)) ?{{ v, match v with MkValConf _ v δ' => Q (MkValConf _ v (env.drop Δ δ')) end }} -∗
-          WP (MkConf (stm_block δΔ k) δ) ?{{ v, Q v }})%I.
-  Proof.
-    iRevert (δ δΔ k Q).
-    iLöb as "IH".
-    iIntros (δ δΔ k Q) "wpk".
-    rewrite ?wp_unfold. cbn.
-    iIntros (σ _ ks1 ks nt) "state_inv".
-    rewrite /wp_pre.
-    destruct (language.to_val (MkConf k (δ ►► δΔ))) eqn:Heqkval.
-    - destruct v as [v δ0]. apply language.of_to_val in Heqkval.
-      inversion Heqkval. subst. clear Heqkval.
-      rewrite env.drop_cat.
-      iMod "wpk" as "H".
-      iMod (fupd_mask_subseteq empty) as "Hclose"; first set_solver.
-      iSplitR; [trivial|].
-      iModIntro.
-      iIntros (e2 σ2 efs) "%".
-      iModIntro. iModIntro. iModIntro.
-      iMod "Hclose" as "e".
-      iDestruct "e" as "_".
-      iModIntro.
-      dependent elimination H.
-      dependent elimination s.
-      + iFrame.
-        iSplitL; [|trivial].
-        by iApply wp_value.
-      + inversion s4.
-    - iMod (fupd_mask_subseteq empty) as "Hclose"; first set_solver.
-      iModIntro.
-      iSplitR; [trivial|].
-      iIntros (e2 σ2 efs2) "%".
-      dependent elimination H.
-      dependent elimination s.
-      + discriminate Heqkval.
-      + iModIntro. iModIntro. iModIntro.
-        iMod "Hclose" as "_".
-        iFrame.
-        iModIntro.
-        iSplitL; [|trivial].
-        iApply wp_compat_fail.
-      + iMod "Hclose" as "_".
-        cbn.
-        iMod ("wpk" $! (γ1 , μ1) 0 nil ks nt with "state_inv") as "[% wpk]".
-        iMod ("wpk" $! _ _ _ (mk_prim_step s4)) as "wpk".
-        iModIntro. iModIntro.
-        iMod "wpk".
-        iModIntro.
-        iMod "wpk" as "[Hregs [wpk' _]]".
-        iModIntro.
-        iFrame.
-        iSplitL; [|trivial].
-        iApply "IH".
-        iFrame.
-  Qed.
-
-  Lemma wp_compat_call_frame {Γ Δ} {τ : Ty} {δ : CStore Γ}
-        (δΔ : CStore Δ) (s : Stm Δ τ) (Q : ValConf Γ τ -> iProp Σ) :
-    ⊢ (WP (MkConf s δΔ) ?{{ v, match v with MkValConf _ v δ' => Q (MkValConf _ v δ) end }} -∗
-          WP (MkConf (stm_call_frame δΔ s) δ) ?{{ v, Q v }})%I.
-  Proof.
-    iRevert (δ δΔ s Q).
-    iLöb as "IH".
-    iIntros (δ δΔ s Q) "wpk".
-    rewrite ?wp_unfold.
-    cbn.
-    iIntros (σ ns ks1 ks nt) "Hregs".
-    iMod (fupd_mask_subseteq empty) as "Hclose"; first set_solver.
-    iModIntro.
-    iSplitR; first trivial.
-    iIntros (e2 σ2 efs) "%".
-    dependent elimination H.
-    dependent elimination s0.
-    - iMod "Hclose" as "_".
-      rewrite {1}/wp_pre.
-      rewrite (val_stuck (MkConf s9 δΔ3) (γ1 , μ1) [] _ _ [] (mk_prim_step s10)).
-      iMod ("wpk" $! (γ1 , μ1) ns nil ks nt with "Hregs") as "[% wpk]". cbn.
-      iMod ("wpk" $! _ _ _ (mk_prim_step s10)) as "wpk".
-      iModIntro. iModIntro.
-      iMod "wpk".
-      iModIntro.
-      iMod "wpk" as "[Hregs [wpk' _]]".
-      iModIntro.
-      iFrame.
-      iSplitL; last trivial.
-      iApply "IH".
-      iFrame.
-    - cbn.
-      iModIntro. iModIntro. iModIntro.
-      iMod "Hclose" as "_".
-      iMod "wpk" as "Qv".
-      iModIntro.
-      iFrame.
-      iSplitL; last trivial.
-      by iApply wp_value.
-    - iModIntro. iModIntro. iModIntro.
-      iMod "Hclose" as "_".
-      iFrame.
-      iModIntro.
-      iSplitL; [|trivial].
-      iApply wp_compat_fail.
-  Qed.
-
-  Definition ValidLemma {Δ} (lem : Lemma Δ) : Prop :=
-    match lem with
-      {| lemma_logic_variables := Σ;
-         lemma_patterns        := θΔ;
-         lemma_precondition    := req;
-         lemma_postcondition   := ens;
-      |} =>
-      forall (ι : Valuation Σ),
-        ⊢ interpret_assertion req ι -∗
-          interpret_assertion ens ι
-    end.
-
-  Fixpoint Forall {Δ : LCtx} {struct Δ} : (Valuation Δ -> iProp Σ) -> iProp Σ :=
-    match Δ return (Valuation Δ -> iProp Σ) -> iProp Σ with
-    | ctx.nil      => fun P => P env.nil
-    | ctx.snoc Δ b => fun P => Forall (fun δ => ∀ (v : Val (type b)), P (env.snoc δ b v))
-    end%I.
-
-  Lemma iris_rule_stm_read_register_wp {Γ τ} (r : 𝑹𝑬𝑮 τ) (v : Val τ) {δ : CStore Γ} :
-    ⊢ (lptsreg r v -∗
-                    WP (MkConf (stm_read_register r) δ) ?{{ w, lptsreg r v ∗ ⌜ w = MkValConf _ v δ ⌝ }}
-      )%I.
-  Proof.
-    iIntros "Hreg".
-    iApply (wp_mask_mono _ empty); auto.
-    rewrite wp_unfold; cbn.
-    iIntros (σ _ ls _ n) "[Hregs Hmem]".
-    iDestruct (@reg_valid with "Hregs Hreg") as %<-.
-    iModIntro.
-    iSplitR; [trivial|].
-    iIntros (e2 σ2 efs) "%".
-    remember (MkConf (stm_read_register r) δ) as t.
-    destruct H as [γ1 γ2 σ1 σ2 δ1 δ2 s1 s2 step].
-    dependent elimination Heqt.
-    destruct (steps_inversion_read_register step) as [<- [<- [<- ->]]].
-    iModIntro. iModIntro. iModIntro.
-    iFrame. iSplitR ""; auto.
-    by iApply wp_value.
-  Qed.
-
-  Lemma iris_rule_stm_write_register_wp {Γ} {τ} (r : 𝑹𝑬𝑮 τ) (δ : CStore Γ) (v : Val τ) e :
-    ⊢ (reg_pointsTo r v -∗
-                    WP (MkConf (stm_write_register r e) δ : expr (microsail_lang Γ τ)) ?{{ w, reg_pointsTo r (eval e δ) ∗ bi_pure (w = MkValConf _ (eval e δ) δ) }}
-    )%I.
-  Proof.
-    iIntros "Hreg".
-    iApply (wp_mask_mono _ empty); auto.
-    rewrite wp_unfold; cbn.
-    iIntros (σ _ ls _ n) "[Hregs Hmem]".
-    iMod (reg_update σ.1 r v (eval e δ) with "Hregs Hreg") as "[Hregs Hreg]".
-    iModIntro.
-    iSplitR; [trivial|].
-    iIntros (e2 σ2 efs) "%".
-    dependent elimination H.
-    destruct (steps_inversion_write_register s) as [-> [<- [<- ->]]].
-    iModIntro. iModIntro. iModIntro.
-    iFrame. iSplitR; auto.
-    by iApply wp_value.
-  Qed.
-
-  Lemma iris_rule_consequence {Γ σ} {δ : CStore Γ}
-        {P P'} {Q Q' : Val σ -> CStore Γ -> iProp Σ} {s : Stm Γ σ} :
-        (P ⊢ P') -> (forall v δ', Q' v δ' ⊢ Q v δ') ->
-        semTriple δ P' s Q' -∗ semTriple δ P s Q.
-  Proof.
-    iIntros (PP QQ) "trips P".
-    iApply (wp_mono _ _ _ (fun v => match v with MkValConf _ v δ' => Q' v δ' end)).
-    + intros [v δ']; cbn.
-      apply QQ.
-    + iApply "trips".
-      iApply PP; iFrame.
-  Qed.
-
-  Lemma iris_rule_frame {Γ σ} {δ : CStore Γ}
-        (R P : iProp Σ) (Q : Val σ -> CStore Γ -> iProp Σ) (s : Stm Γ σ) :
-        (⊢ semTriple δ P s Q -∗ semTriple δ (R ∗ P) s (fun v δ' => R ∗ Q v δ'))%I.
-  Proof.
-    iIntros "trips [HR HP]".
-    iApply (wp_frame_l _ _ (MkConf s δ) (fun v => match v with MkValConf _ v δ' => Q v δ' end) R).
-    iFrame.
-    by iApply "trips".
-  Qed.
-
-  Lemma iris_rule_pull {σ Γ} (δ : CStore Γ) (s : Stm Γ σ)
-        (P : iProp Σ) (Q : Prop) (R : Val σ -> CStore Γ -> iProp Σ) :
-        (⊢ (⌜ Q ⌝ → semTriple δ P s R) -∗ semTriple δ (P ∧ bi_pure Q) s R)%I.
-  Proof.
-    iIntros "QP [P %]".
-    by iApply "QP".
-  Qed.
-
-  Lemma iris_rule_exist {σ Γ} (δ : CStore Γ)
-        (s : Stm Γ σ) {A : Type} {P : A -> iProp Σ}
-        {Q :  Val σ -> CStore Γ -> iProp Σ} :
-        ⊢ ((∀ x, semTriple δ (P x) s Q) -∗ semTriple δ (∃ x, P x) s Q)%I.
-  Proof.
-    iIntros "trips Px".
-    iDestruct "Px" as (x) "Px".
-    by iApply "trips".
-  Qed.
-
-  Lemma iris_rule_stm_val {Γ} (δ : CStore Γ)
-        {τ : Ty} {v : Val τ}
-        {P : iProp Σ} {Q : Val τ -> CStore Γ -> iProp Σ} :
-        ⊢ ((P -∗ Q v δ)%I -∗ semTriple δ P (stm_val τ v) Q)%I.
-  Proof.
-    iIntros "PQ P".
-    iApply wp_value.
-    by iApply "PQ".
-  Qed.
-
-  Lemma iris_rule_stm_exp {Γ} (δ : CStore Γ)
-        {τ : Ty} {e : Exp Γ τ}
-        {P : iProp Σ} {Q : Val τ -> CStore Γ -> iProp Σ} :
-        ⊢ ((P -∗ Q (eval e δ) δ) -∗ semTriple δ P (stm_exp e) Q)%I.
-  Proof.
-    iIntros "PQ P".
-    iApply (wp_mask_mono _ empty); auto.
-    rewrite wp_unfold.
-    iIntros ([regs μ] ns k ks nt) "[Hregs Hmem]".
-    iModIntro.
-    iSplitR; [trivial|].
-    iIntros (e2 σ2 efs) "%".
-    remember (MkConf (stm_exp e) δ) as t.
-    destruct H.
-    dependent elimination Heqt.
-    dependent elimination H.
-    iModIntro. iModIntro. iModIntro.
-    iFrame.
-    iSplitL; cbn; trivial.
-    iApply (wp_value _ _ (fun v => match v with | MkValConf _ v' δ' => Q v' δ' end) (MkConf (stm_val _ (eval e0 δ1)) δ1)).
-    by iApply "PQ".
-  Qed.
-
-  Lemma iris_rule_stm_let {Γ} (δ : CStore Γ)
-        (x : PVar) (σ τ : Ty) (s : Stm Γ σ) (k : Stm (Γ ▻ x∷σ) τ)
-        (P : iProp Σ) (Q : Val σ -> CStore Γ -> iProp Σ)
-        (R : Val τ -> CStore Γ -> iProp Σ) :
-        ⊢ (semTriple δ P s Q -∗
-                     (∀ (v : Val σ) (δ' : CStore Γ),
-                         semTriple (env.snoc δ' (x∷σ) v) (Q v δ') k (fun v δ'' => R v (env.tail δ'')) ) -∗
-                     semTriple δ P (let: x := s in k) R).
-  Proof.
-    iIntros "trips tripk P".
-    iPoseProof ("trips" with "P") as "wpv".
-    iRevert (s δ) "wpv".
-    iLöb as "IH".
-    iIntros (s δ) "wpv".
-    rewrite (wp_unfold _ _ (MkConf (stm_let _ _ _ k) _)). cbn.
-    iIntros ([regs μ] ns ks1 ks nt) "state_inv".
-    iMod (fupd_mask_subseteq empty) as "Hclose"; first set_solver.
-    iModIntro.
-    iSplitR; [trivial|].
-    iIntros (e2 [regs2 μ2] efs) "%".
-    unfold language.prim_step in H; cbn in H.
-    dependent elimination H.
-    dependent elimination s0.
-    + cbn. rewrite wp_unfold. cbn.
-      iModIntro. iModIntro. iModIntro.
-      iMod "Hclose" as "_".
-      iMod "wpv".
-      iPoseProof ("tripk" $! v _ with "wpv") as "wpk".
-      iModIntro.
-      iFrame; iSplitL; auto.
-      by iApply (wp_compat_block (env.snoc env.nil (x0∷σ0) v) _ (fun v0 => match v0 with | MkValConf _ v1 δ' => R v1 δ' end )).
-    + iModIntro. iModIntro. iModIntro.
-      iMod "Hclose" as "_".
-      iFrame; iSplitL; auto.
-      by iApply wp_compat_fail.
-    + cbn.
-      rewrite wp_unfold.
-      unfold wp_pre.
-      rewrite (val_stuck (MkConf s1 δ1) _ [] _ _ [] (mk_prim_step s3)).
-      iSpecialize ("wpv" $! (γ1 , μ1) ns nil nil nt with "state_inv"). cbn.
-      iMod "Hclose" as "_".
-      iMod "wpv" as "[_ wpv]".
-      iSpecialize ("wpv" $! (MkConf s' δ') _ nil (mk_prim_step s3)). cbn.
-      iMod "wpv".
-      iModIntro. iModIntro.
-      iMod "wpv".
-      iModIntro.
-      iMod "wpv" as "[Hregs [wps _]]".
-      iModIntro.
-      iFrame.
-      iSpecialize ("IH" with "tripk").
-      iSpecialize ("IH" with "wps").
-      iFrame.
-  Qed.
-
-  Lemma iris_rule_stm_let_forwards {Γ} (δ : CStore Γ)
-        (x : PVar) (σ τ : Ty) (s : Stm Γ σ) (k : Stm (Γ ▻ x∷σ) τ)
-        (P : iProp Σ) (Q : Val σ -> CStore Γ -> iProp Σ)
-        (R : Val τ -> CStore (Γ ▻ x∷σ) -> iProp Σ) :
-        ⊢ (semTriple δ P s Q -∗
-                     (∀ (v : Val σ) (δ' : CStore Γ), semTriple (env.snoc δ' (x∷σ) v) (Q v δ') k R ) -∗
-                     semTriple δ P (let: x := s in k) (fun v δ' => ∃ v__let, R v (env.snoc δ' (x∷σ) v__let)))%I.
-  Proof.
-    (* proof should be generalizable beyond Iris model? *)
-    iIntros "trips tripk".
-    iApply (iris_rule_stm_let δ s k P Q (fun v δ' => ∃ v__let, R v (env.snoc δ' (x∷σ) v__let))%I with "trips").
-    iIntros (v δ') "Qv".
-    iPoseProof ("tripk" with "Qv") as "wpk".
-    iApply (wp_mono with "wpk").
-    iIntros (v') "Rv".
-    destruct v' as [v0 δ0].
-    iExists (env.head δ0).
-    by dependent elimination δ0.
-  Qed.
-
-  Lemma iris_rule_stm_block {Γ} (δ : CStore Γ)
-        (Δ : PCtx) (δΔ : CStore Δ)
-        (τ : Ty) (k : Stm (Γ ▻▻ Δ) τ)
-        (P : iProp Σ) (R : Val τ -> CStore Γ -> iProp Σ) :
-        ⊢ (semTriple (δ ►► δΔ) P k (fun v δ'' => R v (env.drop Δ δ'')) -∗
-                   semTriple δ P (stm_block δΔ k) R)%I.
-  Proof.
-    iIntros "tripk P".
-    iPoseProof ("tripk" with "P") as "wpk".
-    by iApply (wp_compat_block δΔ k (fun v => match v with | MkValConf _ v' δ' => R v' δ' end) with "wpk").
-  Qed.
-
-  Lemma iris_rule_stm_if {Γ} (δ : CStore Γ)
-        (τ : Ty) (e : Exp Γ ty.bool) (s1 s2 : Stm Γ τ)
-        (P : iProp Σ) (Q : Val τ -> CStore Γ -> iProp Σ) :
-        ⊢ (semTriple δ (P ∧ ⌜ eval e δ = true ⌝) s1 Q -∗
-                   semTriple δ (P ∧ ⌜ eval e δ = false ⌝) s2 Q -∗
-                   semTriple δ P (stm_if e s1 s2) Q)%I.
-  Proof.
-    iIntros "trips1 trips2 P".
-    rewrite wp_unfold. cbn.
-    iIntros (σ _ ks1 ks nt) "Hregs".
-    iMod (fupd_mask_subseteq empty) as "Hclose"; first set_solver.
-    iModIntro. iSplitR; [trivial|].
-    iIntros (e2 σ2 efs) "%".
-    unfold language.prim_step in H; cbn in H.
-    dependent elimination H.
-    dependent elimination s.
-    iModIntro. iModIntro. iModIntro.
-    iMod "Hclose" as "_".
-    iModIntro; iFrame.
-    iSplitL; [|trivial].
-    destruct (eval e1 δ1).
-    - iApply "trips1".
-      by iFrame.
-    - iApply "trips2".
-      by iFrame.
-  Qed.
-
-  Lemma iris_rule_stm_if_backwards {Γ} (δ : CStore Γ)
-        (τ : Ty) (e : Exp Γ ty.bool) (s1 s2 : Stm Γ τ)
-        (P1 P2 : iProp Σ) (Q : Val τ -> CStore Γ -> iProp Σ) :
-        ⊢ (semTriple δ P1 s1 Q -∗ semTriple δ P2 s2 Q -∗
-        semTriple δ (bi_impl (⌜ eval e δ = true ⌝) P1 ∧
-                     bi_impl (⌜ eval e δ = false ⌝) P2)%I
-            (stm_if e s1 s2) Q)%I.
-  Proof.
-    (* generalize proof to non-iris models *)
-    iIntros "trips1 trips2".
-    iApply (iris_rule_stm_if δ e s1 s2
-                             ((⌜ eval e δ = true ⌝ → P1) ∧ (⌜ eval e δ = false ⌝ → P2))%I Q with "[trips1]").
-    - iIntros "[P' %]".
-      iApply "trips1".
-      by iApply (bi.and_elim_l with "P'").
-    - iIntros "[P' %]".
-      iApply "trips2".
-      by iApply (bi.and_elim_r with "P'").
-  Qed.
-
-  Lemma iris_rule_stm_seq {Γ} (δ : CStore Γ)
-        (τ : Ty) (s1 : Stm Γ τ) (σ : Ty) (s2 : Stm Γ σ)
-        (P : iProp Σ) (Q : CStore Γ -> iProp Σ) (R : Val σ -> CStore Γ -> iProp Σ) :
-    ⊢ (semTriple δ P s1 (fun _ => Q) -∗
-                 (∀ δ', semTriple δ' (Q δ') s2 R) -∗
-                 semTriple δ P (s1 ;; s2) R)%I.
-  Proof.
-    iIntros "trips1 trips2 P".
-    iPoseProof ("trips1" with "P") as "wps1".
-    iRevert (s1 δ) "wps1".
-    iLöb as "IH".
-    iIntros (s1 δ) "wps1".
-    rewrite (wp_unfold _ _ (MkConf (stm_seq _ _) _)). cbn.
-    iIntros ([regs μ] ns ks1 ks nt) "Hregs".
-    iMod (fupd_mask_subseteq empty) as "Hclose"; first set_solver.
-    iModIntro.
-    iSplitR; [trivial|].
-    iIntros (e2 σ2 efs) "%".
-    unfold language.prim_step in H; cbn in H.
-    dependent elimination H.
-    dependent elimination s; cbn.
-    + rewrite wp_unfold.
-      unfold wp_pre.
-      rewrite (val_stuck (MkConf s7 δ1) (γ1 , μ1) [] _ _ [] (mk_prim_step s8)).
-      iSpecialize ("wps1" $! (γ1 , μ1) ns nil nil nt with "Hregs"). cbn.
-      iMod "Hclose" as "_".
-      iMod "wps1" as "[_ wps1]". cbn.
-      iMod ("wps1" $! (MkConf s'0 δ'1) _ nil (mk_prim_step s8)) as "wps1".
-      iModIntro. iModIntro. iModIntro.
-      iMod "wps1".
-      iMod "wps1" as "[Hregs [wps' _]]".
-      iFrame.
-      iSplitL; [|trivial].
-      iModIntro.
-      iSpecialize ("IH" with "trips2").
-      by iApply "IH".
-    + rewrite wp_unfold; cbn.
-      iModIntro. iModIntro. iModIntro.
-      iMod "Hclose" as "_".
-      iMod "wps1" as "wps1".
-      iPoseProof ("trips2" $! δ1 with "wps1") as "wps2".
-      by iFrame.
-    + iModIntro. iModIntro. iModIntro.
-      iMod "Hclose" as "_".
-      iFrame; iSplitL; auto.
-      by iApply wp_compat_fail.
-  Qed.
-
-  Lemma iris_rule_stm_assertk {Γ τ} (δ : CStore Γ)
-        (e1 : Exp Γ ty.bool) (e2 : Exp Γ ty.string) (k : Stm Γ τ)
-                      (P : iProp Σ) (Q : Val τ -> CStore Γ -> iProp Σ) :
-    ⊢ (semTriple δ (P ∧ ⌜ eval e1 δ = true ⌝) k Q -∗
-       semTriple δ P (stm_assertk e1 e2 k) Q)%I.
-  Proof.
-    iIntros "tripk P".
-    rewrite wp_unfold. cbn.
-    iIntros (σ ns ks1 ks nt) "Hregs".
-    iMod (fupd_mask_subseteq empty) as "Hclose"; first set_solver.
-    iModIntro. iSplitR; [trivial|].
-    iIntros (e3 σ2 efs) "%".
-    unfold language.prim_step in H; cbn in H.
-    dependent elimination H.
-    dependent elimination s.
-    iModIntro. iModIntro. iModIntro.
-    iMod "Hclose" as "_".
-    iModIntro; iFrame.
-    iSplitL; [|trivial].
-    destruct (eval e3 δ1) eqn:Heqc.
-    - iApply "tripk".
-      by iFrame.
-    - iApply wp_compat_fail.
-  Qed.
-
-  Lemma iris_rule_stm_fail {Γ} (δ : CStore Γ)
-        (τ : Ty) (s : Val ty.string) :
-        forall (Q : Val τ -> CStore Γ -> iProp Σ),
-          ⊢ semTriple δ True%I (stm_fail τ s) Q.
-  Proof.
-    iIntros (Q) "_".
-    iApply wp_compat_fail.
-  Qed.
-
-  Lemma iris_rule_stm_match_list {Γ} (δ : CStore Γ)
-        {σ τ : Ty} (e : Exp Γ (ty.list σ)) (alt_nil : Stm Γ τ)
-        (xh xt : PVar) (alt_cons : Stm (Γ ▻ xh∷σ ▻ xt∷ty.list σ) τ)
-        (P : iProp Σ) (Q : Val τ -> CStore Γ -> iProp Σ) :
-        ⊢ (semTriple δ (P ∧ bi_pure (eval e δ = []%list)) alt_nil (fun v' δ' => Q v' δ') -∗
-                     (∀ v vs, semTriple (env.snoc (env.snoc δ (xh∷σ) v) (xt∷ty.list σ) vs) (P ∧ bi_pure (eval e δ = cons v vs)) alt_cons (fun v' δ' => Q v' (env.tail (env.tail δ')))) -∗
-                     semTriple δ P (stm_match_list e alt_nil xh xt alt_cons) Q)%I.
-  Proof.
-    iIntros "tripnil tripcons P".
-    rewrite wp_unfold. cbn.
-    iIntros (σ1 _ ks1 ks nt) "Hregs".
-    iMod (fupd_mask_subseteq empty) as "Hclose"; first set_solver.
-    iModIntro. iSplitR; [trivial|].
-    iIntros (e3 σ2 efs) "%".
-    unfold language.prim_step in H; cbn in H.
-    dependent elimination H.
-    dependent elimination s.
-    remember (eval e4 δ1) as scrutinee.
-    destruct scrutinee as [|l ls].
-    - iModIntro. iModIntro. iModIntro.
-      iMod "Hclose" as "_".
-      iModIntro. iFrame.
-      iSplitL; [|trivial].
-      iApply "tripnil".
-      by iFrame.
-    - iModIntro. iModIntro. iModIntro.
-      iMod "Hclose" as "_".
-      iModIntro.
-      iFrame.
-      iSplitL; [|trivial].
-      iApply (wp_compat_block (env.snoc (env.snoc env.nil (xh0∷σ6) l) (xt0∷ty.list σ6) ls)).
-      iApply "tripcons".
-      by iFrame.
-  Qed.
-
-  Lemma iris_rule_stm_match_sum {Γ} (δ : CStore Γ)
-        (σinl σinr τ : Ty) (e : Exp Γ (ty.sum σinl σinr))
-                         (xinl : PVar) (alt_inl : Stm (Γ ▻ xinl∷σinl) τ)
-                         (xinr : PVar) (alt_inr : Stm (Γ ▻ xinr∷σinr) τ)
-                         (P : iProp Σ)
-                         (Q : Val τ -> CStore Γ -> iProp Σ) :
-        ⊢ ((∀ v, semTriple (env.snoc δ (xinl∷σinl) v) (P ∧ ⌜ eval e δ = inl v ⌝) alt_inl (fun v' δ' => Q v' (env.tail δ'))) -∗
-           (∀ v, semTriple (env.snoc δ (xinr∷σinr) v) (P ∧ ⌜ eval e δ = inr v ⌝) alt_inr (fun v' δ' => Q v' (env.tail δ'))) -∗
-        semTriple δ P (stm_match_sum e xinl alt_inl xinr alt_inr) Q)%I.
-  Proof.
-    iIntros "tripinl tripinr P".
-    rewrite wp_unfold. cbn.
-    iIntros (σ1 _ ks1 ks nt) "Hregs".
-    iMod (fupd_mask_subseteq empty) as "Hclose"; first set_solver.
-    iModIntro. iSplitR; [trivial|].
-    iIntros (e2 σ2 efs) "%".
-    unfold language.prim_step in H; cbn in H.
-    dependent elimination H.
-    dependent elimination s.
-    remember (eval e5 δ1) as scrutinee.
-    destruct scrutinee as [v1|v2].
-    - iModIntro. iModIntro. iModIntro.
-      iMod "Hclose" as "_".
-      iModIntro. iFrame.
-      iSplitL; [|trivial].
-      iApply (wp_compat_block (env.snoc env.nil (xinl0∷σinl0) v1)).
-      iApply ("tripinl" $! v1).
-      by iFrame.
-    - iModIntro. iModIntro. iModIntro.
-      iMod "Hclose" as "_".
-      iModIntro. iFrame.
-      iSplitL; [|trivial].
-      iApply (wp_compat_block (env.snoc env.nil (xinr0∷σinr0) v2)).
-      iApply ("tripinr" $! v2).
-      by iFrame.
-  Qed.
-
-  Lemma iris_rule_stm_match_prod {Γ} (δ : CStore Γ)
-        {σ1 σ2 τ : Ty} (e : Exp Γ (ty.prod σ1 σ2))
-        (xl xr : PVar) (rhs : Stm (Γ ▻ xl∷σ1 ▻ xr∷σ2) τ)
-        (P : iProp Σ) (Q : Val τ -> CStore Γ -> iProp Σ) :
-        ⊢ ((∀ vl vr,
-            semTriple (env.snoc (env.snoc δ (xl∷σ1) vl) (xr∷σ2) vr)
-              (P ∧ bi_pure (eval e δ = (vl,vr))) rhs (fun v δ' => Q v (env.tail (env.tail δ')))) -∗
-          semTriple δ P (stm_match_prod e xl xr rhs) Q)%I.
-  Proof.
-    iIntros "trippair P".
-    rewrite wp_unfold. cbn.
-    iIntros (σ _ ks1 ks nt) "Hregs".
-    iMod (fupd_mask_subseteq empty) as "Hclose"; first set_solver.
-    iModIntro. iSplitR; [trivial|].
-    iIntros (e2 σ' efs) "%".
-    unfold language.prim_step in H; cbn in H.
-    dependent elimination H.
-    dependent elimination s.
-    remember (eval e6 δ1) as scrutinee.
-    destruct scrutinee as [v1 v2].
-    iModIntro. iModIntro. iModIntro.
-    iMod "Hclose" as "_".
-    iModIntro. iFrame.
-    iSplitL; [|trivial].
-    iApply (wp_compat_block (env.snoc (env.snoc env.nil (xl0∷σ8) v1) (xr0∷σ9) v2)).
-    iApply ("trippair" $! v1 v2).
-    by iFrame.
-  Qed.
-
-  Lemma iris_rule_stm_match_enum {Γ} (δ : CStore Γ)
-        {E : enumi} (e : Exp Γ (ty.enum E)) {τ : Ty}
-        (alts : forall (K : enumt E), Stm Γ τ)
-        (P : iProp Σ) (Q : Val τ -> CStore Γ -> iProp Σ) :
-        ⊢ (semTriple δ P (alts (eval e δ)) Q -∗
-          semTriple δ P (stm_match_enum E e alts) Q)%I.
-  Proof.
-    iIntros "tripalt P".
-    rewrite wp_unfold. cbn.
-    iIntros (σ _ ks1 ks nt) "Hregs".
-    iMod (fupd_mask_subseteq empty) as "Hclose"; first set_solver.
-    iModIntro. iSplitR; [trivial|].
-    iIntros (e2 σ' efs) "%".
-    unfold language.prim_step in H; cbn in H.
-    dependent elimination H.
-    dependent elimination s.
-    iModIntro. iModIntro. iModIntro.
-    iMod "Hclose" as "_".
-    iModIntro. iFrame.
-    iSplitL; [|trivial].
-    by iApply "tripalt".
-  Qed.
-
-  Lemma iris_rule_stm_match_tuple {Γ} (δ : CStore Γ)
-        {σs : Ctx Ty} {Δ : PCtx} (e : Exp Γ (ty.tuple σs))
-        (p : TuplePat σs Δ) {τ : Ty} (rhs : Stm (Γ ▻▻ Δ) τ)
-        (P : iProp Σ) (Q : Val τ -> CStore Γ -> iProp Σ) :
-    ⊢ ((semTriple (env.cat δ (tuple_pattern_match_val p (eval e δ))) P rhs (fun v δ' => Q v (env.drop Δ δ'))) -∗
-       semTriple δ P (stm_match_tuple e p rhs) Q)%I.
-  Proof.
-    iIntros "triptup P".
-    rewrite wp_unfold. cbn.
-    iIntros (σ ns ks1 ks nt) "Hregs".
-    iMod (fupd_mask_subseteq empty) as "Hclose"; first set_solver.
-    iModIntro. iSplitR; [trivial|].
-    iIntros (e2 σ' efs) "%".
-    unfold language.prim_step in H; cbn in H.
-    dependent elimination H.
-    dependent elimination s.
-    iModIntro. iModIntro. iModIntro.
-    iMod "Hclose" as "_".
-    iModIntro. iFrame.
-    iSplitL; [|trivial].
-    iApply (wp_compat_block (tuple_pattern_match_val p0 (eval e8 δ1))).
-    by iApply "triptup".
-  Qed.
-
-  Lemma iris_rule_stm_match_union {Γ} (δ : CStore Γ)
-        {U : unioni} (e : Exp Γ (ty.union U)) {σ τ : Ty}
-        (alt__Δ : forall (K : unionk U), PCtx)
-        (alt__p : forall (K : unionk U), Pattern (alt__Δ K) (unionk_ty U K))
-        (alt__r : forall (K : unionk U), Stm (Γ ▻▻ alt__Δ K) τ)
-        (P : iProp Σ) (Q : Val τ -> CStore Γ -> iProp Σ) :
-        ⊢ ((∀ (K : unionk U) (v : Val (unionk_ty U K)),
-               semTriple (env.cat δ (pattern_match_val (alt__p K) v)) (P ∧ bi_pure (eval e δ = unionv_fold U (existT K v))) (alt__r K) (fun v δ' => Q v (env.drop (alt__Δ K) δ'))) -∗
-               semTriple δ P (stm_match_union U e alt__p alt__r) Q
-          )%I.
-  Proof.
-    iIntros "tripunion P".
-    rewrite wp_unfold. cbn.
-    iIntros (σ1 ns ks1 ks nt) "Hregs".
-    iMod (fupd_mask_subseteq empty) as "Hclose"; first set_solver.
-    iModIntro. iSplitR; [trivial|].
-    iIntros (e2 σ2 efs) "%".
-    unfold language.prim_step in H; cbn in H.
-    dependent elimination H.
-    dependent elimination s.
-    iModIntro. iModIntro. iModIntro.
-    iMod "Hclose" as "_".
-    iModIntro. iFrame.
-    iSplitL; [|trivial].
-    remember (unionv_unfold U0 (eval e9 δ1)) as scrutinee.
-    destruct scrutinee as [K v].
-    iApply (wp_compat_block (pattern_match_val (alt__pat K) v)).
-    iSpecialize ("tripunion" $! K v).
-    rewrite Heqscrutinee.
-    rewrite unionv_fold_unfold.
-    iApply "tripunion".
-    by iFrame.
-  Qed.
-
-  Lemma iris_rule_stm_match_record {Γ} (δ : CStore Γ)
-        {R : recordi} {Δ : PCtx} (e : Exp Γ (ty.record R))
-        (p : RecordPat (recordf_ty R) Δ) {τ : Ty} (rhs : Stm (Γ ▻▻ Δ) τ)
-        (P : iProp Σ) (Q : Val τ -> CStore Γ -> iProp Σ) :
-        ⊢ ((semTriple (env.cat δ (record_pattern_match_val p (eval e δ))) P rhs (fun v δ' => Q v (env.drop Δ δ'))) -∗
-        semTriple δ P (stm_match_record R e p rhs) Q)%I.
-  Proof.
-    iIntros "triprec P".
-    rewrite wp_unfold. cbn.
-    iIntros (σ1 ns ks1 ks nt) "Hregs".
-    iMod (fupd_mask_subseteq empty) as "Hclose"; first set_solver.
-    iModIntro. iSplitR; [trivial|].
-    iIntros (e2 σ2 efs) "%".
-    unfold language.prim_step in H; cbn in H.
-    dependent elimination H.
-    dependent elimination s.
-    iModIntro. iModIntro. iModIntro.
-    iMod "Hclose" as "_".
-    iModIntro. iFrame.
-    iSplitL; [|trivial].
-    iApply (wp_compat_block (record_pattern_match_val p1 (eval e10 δ1))).
-    by iApply "triprec".
-  Qed.
-
-  Lemma iris_rule_stm_match_bvec {Γ} (δ : CStore Γ)
-        {n : nat} (e : Exp Γ (ty.bvec n)) {τ : Ty}
-        (rhs : forall (v : bv n), Stm Γ τ)
-        (P : iProp Σ) (Q : Val τ -> CStore Γ -> iProp Σ) :
-        ⊢ (semTriple δ P (rhs (eval e δ)) Q -∗
-          semTriple δ P (stm_match_bvec n e rhs) Q)%I.
-  Proof.
-    iIntros "triprhs P".
-    rewrite wp_unfold. cbn.
-    iIntros (σ _ ks1 ks nt) "Hregs".
-    iMod (fupd_mask_subseteq empty) as "Hclose"; first set_solver.
-    iModIntro. iSplitR; [trivial|].
-    iIntros (e2 σ' efs) "%".
-    unfold language.prim_step in H; cbn in H.
-    dependent elimination H.
-    dependent elimination s.
-    iModIntro. iModIntro. iModIntro.
-    iMod "Hclose" as "_".
-    iModIntro. iFrame.
-    iSplitL; [|trivial].
-    by iApply "triprhs".
-  Qed.
-
-  Lemma iris_rule_stm_read_register {Γ} (δ : CStore Γ)
-        {σ : Ty} (r : 𝑹𝑬𝑮 σ) (v : Val σ) :
-        ⊢ (semTriple δ (lptsreg r v) (stm_read_register r) (fun v' δ' => ⌜ δ' = δ ⌝ ∧ ⌜ v' = v ⌝ ∧ lptsreg r v))%I.
-  Proof.
-    iIntros "Hreg".
-    iApply wp_mono; [| iApply (iris_rule_stm_read_register_wp with "Hreg") ].
-    iIntros ([δ' v']) "[Hreg %]".
-    inversion H.
-    by iFrame.
-  Qed.
-
-  Lemma iris_rule_stm_write_register {Γ} (δ : CStore Γ)
-        {σ : Ty} (r : 𝑹𝑬𝑮 σ) (w : Exp Γ σ)
-                              (Q : Val σ -> CStore Γ -> iProp Σ)
-                              (v : Val σ) :
-        ⊢ semTriple δ (lptsreg r v) (stm_write_register r w)
-                  (fun v' δ' => ⌜δ' = δ⌝ ∧ ⌜v' = eval w δ⌝ ∧ lptsreg r v')%I.
-  Proof.
-    iIntros "Hreg".
-    iApply wp_mono; [|iApply (iris_rule_stm_write_register_wp with "Hreg")].
-    iIntros (v') "[Hreg %]".
-    rewrite H.
-    by iFrame.
-  Qed.
-
-  Lemma iris_rule_stm_assign_forwards {Γ} (δ : CStore Γ)
-        (x : PVar) (σ : Ty) (xIn : x∷σ ∈ Γ) (s : Stm Γ σ)
-        (P : iProp Σ) (R : Val σ -> CStore Γ -> iProp Σ) :
-        ⊢ (semTriple δ P s R -∗
-                     semTriple δ P (stm_assign x s) (fun v__new δ' => ∃ v__old, R v__new (@env.update _ _ _ δ' (x∷_)  _ v__old) ∧ bi_pure (env.lookup δ' xIn = v__new)))%I.
-  Proof.
-    iIntros "trips P".
-    iPoseProof ("trips" with "P") as "wpv".
-    iRevert (s δ) "wpv".
-    iLöb as "IH".
-    iIntros (s δ) "wpv".
-    rewrite (wp_unfold _ _ (MkConf (stm_assign _ s) _)). cbn.
-    iIntros ([regs μ] ns ks1 ks nt) "Hregs".
-    iMod (fupd_mask_subseteq empty) as "Hclose"; first set_solver.
-    iModIntro.
-    iSplitR; [trivial|].
-    iIntros (e2 [regs2 μ2] efs) "%".
-    unfold language.prim_step in H; cbn in H.
-    dependent elimination H.
-    dependent elimination s0.
-    cbn.
-    + rewrite wp_unfold; cbn.
-      iModIntro. iModIntro. iModIntro.
-      iMod "Hclose" as "_".
-      iMod "wpv" as "wpv".
-      iModIntro.
-      iFrame.
-      iSplitL; [|trivial].
-      iApply wp_value.
-      cbn.
-      iExists (env.lookup δ1 xInΓ).
-      rewrite env.update_update env.update_lookup env.lookup_update.
-      by iFrame.
-    + iModIntro. iModIntro. iModIntro.
-      iMod "Hclose" as "_".
-      cbn.
-      iFrame; iSplitL; auto.
-      by iApply wp_compat_fail.
-    + rewrite wp_unfold.
-      unfold wp_pre.
-      rewrite (val_stuck (MkConf s13 δ1) _ [] _ _ [] (mk_prim_step s14)).
-      iSpecialize ("wpv" $! _ ns nil nil nt with "Hregs"). cbn.
-      iMod "Hclose".
-      iMod "wpv" as "[_ wpv]".
-      iSpecialize ("wpv" $! _ _ nil (mk_prim_step s14)).
-      iMod "wpv" as "wpv".
-      iModIntro. iModIntro.
-      iMod "wpv".
-      iModIntro.
-      iMod "wpv" as "[Hregs [wps _]]".
-      iModIntro.
-      iFrame.
-      by iApply "IH".
-  Qed.
-
-  Lemma iris_rule_stm_assign_backwards {Γ} (δ : CStore Γ)
-        (x : PVar) (σ : Ty) (xIn : x∷σ ∈ Γ) (s : Stm Γ σ)
-        (P : iProp Σ) (R : Val σ -> CStore Γ -> iProp Σ) :
-        ⊢ (semTriple δ P s (fun v δ' => R v (@env.update _ _ _ δ' (x∷_) _ v)) -∗
-           semTriple δ P (stm_assign x s) R)%I.
-  Proof.
-    iIntros "trips P".
-    iPoseProof (iris_rule_stm_assign_forwards _ with "trips P") as "wpas".
-    iApply (wp_mono with "wpas").
-    iIntros ([v' δ']) "Rv".
-    iDestruct "Rv" as (v__old) "[Rv %]".
-    rewrite <-H.
-    by rewrite env.update_update env.update_lookup.
-  Qed.
-
-  Lemma iris_rule_stm_bind {Γ} (δ : CStore Γ)
-        {σ τ : Ty} (s : Stm Γ σ) (k : Val σ -> Stm Γ τ)
-        (P : iProp Σ) (Q : Val σ -> CStore Γ -> iProp Σ)
-        (R : Val τ -> CStore Γ -> iProp Σ) :
-        ⊢ (semTriple δ P s Q -∗
-           (∀ (v__σ : Val σ) (δ' : CStore Γ),
-               semTriple δ' (Q v__σ δ') (k v__σ) R) -∗
-           semTriple δ P (stm_bind s k) R)%I.
-  Proof.
-    iIntros "trips tripk P".
-    iPoseProof ("trips" with "P") as "wpv".
-    iRevert (s δ) "wpv".
-    iLöb as "IH".
-    iIntros (s δ) "wpv".
-    rewrite (wp_unfold _ _ (MkConf (stm_bind _ k) _)). cbn.
-    iIntros ([regs μ] ns ks1 ks nt) "Hregs".
-    iMod (fupd_mask_subseteq empty) as "Hclose"; first set_solver.
-    iModIntro.
-    iSplitR; [trivial|].
-    iIntros (e2 [regs2 μ2] efs) "%".
-    unfold language.prim_step in H; cbn in H.
-    dependent elimination H.
-    dependent elimination s0.
-    + rewrite wp_unfold. cbn.
-      unfold wp_pre.
-      rewrite (val_stuck (MkConf s17 δ1) (γ1 , μ1) [] _ _ [] (mk_prim_step s18)).
-      iSpecialize ("wpv" $! (γ1 , μ1) ns nil nil nt with "Hregs"). cbn.
-      iMod "Hclose".
-      iMod "wpv" as "[_ wpv]".
-      iSpecialize ("wpv" $! _ _ nil (mk_prim_step s18)).
-      iMod "wpv" as "wpv".
-      iModIntro. iModIntro.
-      iMod "wpv".
-      iModIntro.
-      iMod "wpv" as "[Hregs [wps _]]".
-      iModIntro.
-      iFrame.
-      iApply ("IH" with "tripk wps").
-    + iModIntro. iModIntro. iModIntro.
-      iMod "Hclose" as "_".
-      rewrite wp_unfold; cbn.
-      iMod "wpv" as "wpv".
-      iPoseProof ("tripk" with "wpv") as "wpk".
-      iModIntro.
-      by iFrame.
-    + iModIntro. iModIntro. iModIntro.
-      iMod "Hclose" as "_".
-      cbn.
-      iFrame; iSplitL; auto.
-      by iApply wp_compat_fail.
-  Qed.
-
-  Lemma iris_rule_stm_call_inline_later
-    {Γ} (δ : CStore Γ)
-    {Δ σ} (f : 𝑭 Δ σ) (es : NamedEnv (Exp Γ) Δ)
-    (P : iProp Σ) (Q : Val σ -> iProp Σ) :
-    ⊢ ▷ semTriple (evals es δ) P (FunDef f) (fun v _ => Q v) -∗
-      semTriple δ P (stm_call f es) (fun v δ' => Q v ∧ bi_pure (δ = δ')).
-  Proof.
-    iIntros "tripbody P".
-    rewrite wp_unfold. cbn.
-    iIntros (σ' ns ks1 ks nt) "Hregs".
-    iMod (fupd_mask_subseteq empty) as "Hclose"; first set_solver.
-    iModIntro. iSplitR; [trivial|].
-    iIntros (e2 σ'' efs) "%".
-    dependent elimination H.
-    dependent elimination s.
-    iModIntro. iModIntro. iModIntro.
-    iMod "Hclose" as "_".
-    iModIntro. iFrame.
-    iSplitL; [|trivial].
-    iApply wp_compat_call_frame.
-    iApply (wp_mono _ _ _ (fun v => Q (valconf_val v))).
-    { iIntros ([σ' v]) "Qv".
-      by iFrame.
-    }
-    iApply ("tripbody" with "P").
-  Qed.
-
-  Lemma iris_rule_stm_call_inline
-    {Γ} (δ : CStore Γ)
-    {Δ σ} (f : 𝑭 Δ σ) (es : NamedEnv (Exp Γ) Δ)
-    (P : iProp Σ) (Q : Val σ -> iProp Σ) :
-    ⊢ semTriple (evals es δ) P (FunDef f) (fun v _ => Q v) -∗
-      semTriple δ P (stm_call f es) (fun v δ' => Q v ∧ bi_pure (δ = δ')).
-  Proof.
-    iIntros "Hdef".
-    iApply (iris_rule_stm_call_inline_later with "Hdef").
-  Qed.
-
-  Lemma iris_rule_stm_debugk
-    {Γ τ} (δ : CStore Γ) (k : Stm Γ τ)
-    (P : iProp Σ) (Q : Val τ -> CStore Γ -> iProp Σ) :
-    ⊢ (semTriple δ P k Q -∗
-       semTriple δ P (stm_debugk k) Q)%I.
-  Proof.
-    iIntros "tripk P".
-    rewrite wp_unfold. cbn.
-    iIntros (σ ns ks1 ks nt) "Hregs".
-    iMod (fupd_mask_subseteq empty) as "Hclose"; first set_solver.
-    iModIntro. iSplitR; [trivial|].
-    iIntros (e3 σ2 efs) "%".
-    dependent elimination H.
-    dependent elimination s.
-    iModIntro. iModIntro. iModIntro.
-    iMod "Hclose" as "_".
-    iModIntro; iFrame.
-    iSplitL; [|trivial].
-    iApply "tripk".
-    by iFrame.
-  Qed.
-
-  Lemma iris_rule_noop {Γ σ} {δ : CStore Γ}
-        {P} {Q : Val σ -> CStore Γ -> iProp Σ} {s : Stm Γ σ} :
-    language.to_val (MkConf s δ) = None ->
-    (forall {s' γ γ' μ μ' δ'}, ⟨ γ, μ, δ, s ⟩ ---> ⟨ γ', μ', δ', s' ⟩ ->
-                            (γ' = γ) /\ (μ' = μ) /\ (δ' = δ) /\
-                            ((exists v, s' = stm_val _ v) \/ (exists msg, s' = stm_fail _ msg))) ->
-    (∀ v, P ={⊤}=∗ Q v δ) -∗
-                 semTriple δ P s Q.
-  Proof.
-    iIntros (Hnv Hnoop) "HPQ HP".
-    rewrite wp_unfold.
-    unfold wp_pre.
-    rewrite Hnv. cbn.
-    iIntros (σ' ns ks1 ks nt) "Hregs".
-    iMod (fupd_mask_subseteq empty) as "Hclose"; first set_solver.
-    iModIntro.
-    iSplitR; first done.
-    iIntros (e2 σ'' efs) "%".
-    dependent elimination H.
-    destruct (Hnoop _ _ _ _ _ _ s0) as (-> & -> & -> & [[v ->]|[msg ->]]).
-    - do 3 iModIntro.
-      iMod "Hclose" as "_".
-      iMod ("HPQ" with "HP") as "HQ".
-      iModIntro.
-      iFrame.
-      iSplitL; trivial.
-      now iApply wp_value.
-    - do 3 iModIntro.
-      iMod "Hclose" as "_".
-      iModIntro.
-      iFrame.
-      iSplitL; trivial.
-      now iApply wp_compat_fail.
-  Qed.
-
-  Definition ValidContractSemCurried {Δ σ} (body : Stm Δ σ) (contract : SepContract Δ σ) : iProp Σ :=
-    match contract with
-    | MkSepContract _ _ ctxΣ θΔ pre result post =>
-      Forall (fun (ι : Valuation ctxΣ) =>
-        semTriple (inst θΔ ι) (interpret_assertion pre ι) body
-                  (fun v δ' => interpret_assertion post (env.snoc ι (result∷σ) v)))
-    end%I.
-
-  Definition ValidContractSem {Δ σ} (body : Stm Δ σ) (contract : SepContract Δ σ) : iProp Σ :=
-    match contract with
-    | MkSepContract _ _ ctxΣ θΔ pre result post =>
-      ∀ (ι : Valuation ctxΣ),
-        semTriple (inst θΔ ι) (interpret_assertion pre ι) body
-                  (fun v δ' => interpret_assertion post (env.snoc ι (result∷σ) v))
-    end%I.
-
-End Soundness.
-
-Section Adequacy.
-
-  Import SmallStepNotations.
-
-  Definition sailΣ : gFunctors := #[ memΣ ; invΣ ; GFunctor regUR].
-
-  Instance subG_sailGpreS {Σ} : subG sailΣ Σ -> sailGpreS Σ.
-  Proof.
-    intros.
-    lazymatch goal with
-    | H:subG ?xΣ _ |- _ => try unfold xΣ in H
-    end.
-    repeat match goal with
-           | H:subG (gFunctors.app _ _) _ |- _ => apply subG_inv in H; destruct H
-           end.
-    split; eauto using memΣ_GpreS, subG_invΣ.
-    solve_inG.
- Qed.
-
-  Definition RegStore_to_map (γ : RegStore) : gmap SomeReg (exclR (leibnizO SomeVal)) :=
-    list_to_map (K := SomeReg)
-                (fmap (fun x => match x with
-                              existT _ r =>
-                                pair (existT _ r) (Excl (existT _ (read_register γ r)))
-                            end)
-                     (finite.enum (sigT 𝑹𝑬𝑮))).
-
-  Lemma RegStore_to_map_Forall (γ : RegStore) :
-    map_Forall (K := SomeReg)
-      (fun reg v => match reg with | existT _ reg => Excl (existT _ (read_register γ reg)) = v end)
-      (RegStore_to_map γ).
-  Proof.
-    eapply map_Forall_lookup_2.
-    intros [σ r] x eq.
-    unfold RegStore_to_map in eq.
-    remember (list_to_map _ !! _) as o in eq.
-    destruct o; inversion eq; subst.
-    assert (eq' := eq_sym Heqo).
-    rewrite <-elem_of_list_to_map in eq'.
-    - eapply elem_of_list_fmap_2 in eq'.
-      destruct eq' as ([σ' r'] & eq2 & eq3).
-      now inversion eq2.
-    - rewrite <-list_fmap_compose.
-      rewrite (list_fmap_ext (compose fst (λ x : {H : Ty & 𝑹𝑬𝑮 H},
-          let (x0, r0) := x in (existT x0 r0 , Excl (existT x0 (read_register γ r0))))) id _ _ _ eq_refl).
-      + rewrite list_fmap_id.
-        eapply finite.NoDup_enum.
-      + now intros [σ' r'].
-  Qed.
-
-  Lemma RegStore_to_map_valid (γ : RegStore) :
-    valid (RegStore_to_map γ).
-  Proof.
-    intros i.
-    cut (exists v, RegStore_to_map γ !! i = Some (Excl v)).
-    - intros [v eq].
-      now rewrite eq.
-    - destruct i as [σ r].
-      exists (existT _ (read_register γ r)).
-      eapply elem_of_list_to_map_1'.
-      + intros y eq.
-        eapply elem_of_list_fmap_2 in eq.
-        destruct eq as ([σ2 r2] & eq1 & eq2).
-        now inversion eq1.
-      + refine (elem_of_list_fmap_1 _ _ (existT _ r) _).
-        eapply finite.elem_of_enum.
-  Qed.
-
-  Lemma steps_to_erased {σ Γ γ μ δ} (s : Stm Γ σ) {γ' μ' δ' s'}:
-    ⟨ γ, μ, δ, s ⟩ --->* ⟨ γ', μ', δ', s' ⟩ ->
-    rtc erased_step (cons (MkConf s δ) nil, (γ,μ)) (cons (MkConf s' δ') nil, (γ',μ')).
-  Proof.
-    induction 1; first done.
-    refine (rtc_l _ _ _ _ _ IHSteps).
-    exists nil.
-    refine (step_atomic _ _ _ _ _ nil nil eq_refl eq_refl _).
-    by eapply mk_prim_step.
-  Qed.
-
-  Lemma own_RegStore_to_map_reg_pointsTos `{sailRegGS Σ'} {γ : RegStore} {l : list (sigT 𝑹𝑬𝑮)} :
-    NoDup l ->
-    ⊢ own reg_gv_name (◯ list_to_map (K := SomeReg)
-                         (fmap (fun x => match x with existT _ r =>
-                                                     pair (existT _ r) (Excl (existT _ (read_register γ r)))
-                                      end) l)) -∗
-      [∗ list] x ∈ l,
-        let (x0, r) := (x : sigT 𝑹𝑬𝑮) in reg_pointsTo r (read_register γ r).
-  Proof.
-    iIntros (nodups) "Hregs".
-    iInduction l as [|[x r]] "IH".
-    - now iFrame.
-    - rewrite big_sepL_cons. cbn.
-      rewrite (insert_singleton_op (A := exclR (leibnizO SomeVal)) (list_to_map (_ <$> l))  (existT x r) (Excl (existT _ (read_register γ r)))).
-      rewrite auth_frag_op.
-      iPoseProof (own_op with "Hregs") as "[Hreg Hregs]".
-      iFrame.
-      iApply "IH".
-      + iPureIntro.
-        refine (NoDup_cons_1_2 (existT x r) l nodups).
-      + iFrame.
-      + destruct (proj1 (NoDup_cons (existT x r) _) nodups) as [notin _].
-        refine (not_elem_of_list_to_map_1 _ (existT x r) _).
-        rewrite <-list_fmap_compose.
-        rewrite (list_fmap_ext (compose fst (λ x : {H : Ty & 𝑹𝑬𝑮 H},
-          let (x0, r0) := x in (existT x0 r0, Excl (existT x0 (read_register γ r0))))) id _ _ _ eq_refl).
-        now rewrite list_fmap_id.
-        now intros [σ2 r2].
-  Qed.
-
-  Lemma adequacy {Γ σ} (s : Stm Γ σ) {γ γ'} {μ μ'}
-        {δ δ' : CStore Γ} {s' : Stm Γ σ} {Q : Val σ -> Prop} :
-    ⟨ γ, μ, δ, s ⟩ --->* ⟨ γ', μ', δ', s' ⟩ -> Final s' ->
-    (forall `{sailGS Σ'},
-        ⊢ semTriple (Σ := Σ') δ
-          (mem_res sailGS_memGS μ ∗
-           [∗ list] _ ↦ x ∈ finite.enum (sigT 𝑹𝑬𝑮),
-              match x with | existT _ r => reg_pointsTo r (read_register γ r) end
-          )%I s (fun v δ' => bi_pure (Q v)))%I ->
-    ResultOrFail s' Q.
-  Proof.
-    intros steps fins trips.
-    cut (adequate MaybeStuck (MkConf s δ) (γ,μ)
-             (λ (v : val (microsail_lang Γ σ)) (_ : state (microsail_lang Γ σ)),
-                (λ v0 : val (microsail_lang Γ σ), match v0 with
-                                                  | MkValConf _ v' _ => Q v'
-                                                  end) v)).
-    - destruct s'; cbn in fins; destruct fins; last done.
-      intros adeq.
-      apply (adequate_result MaybeStuck (MkConf s δ) (γ , μ) (fun v _ => match v with | MkValConf _ v' δ' => Q v' end) adeq nil (γ' , μ') (MkValConf _ v δ')).
-      by apply steps_to_erased.
-    - constructor; last done.
-      intros t2 σ2 [v2 δ2] eval.
-      assert (eq := RegStore_to_map_Forall γ).
-      assert (regsmapv := RegStore_to_map_valid γ).
-      pose proof (wp_adequacy sailΣ (microsail_lang Γ σ) MaybeStuck (MkConf s δ) (γ , μ) (fun v => match v with | MkValConf _ v' δ' => Q v' end)) as adeq.
-      refine (adequate_result _ _ _ _ (adeq _) _ _ _ eval); clear adeq.
-      iIntros (Hinv κs) "".
-      iMod (own_alloc ((● RegStore_to_map γ ⋅ ◯ RegStore_to_map γ ) : regUR)) as (spec_name) "[Hs1 Hs2]";
-        first by apply auth_both_valid.
-      pose proof (memΣ_GpreS (Σ := sailΣ) _) as mPG.
-      iMod (mem_inv_init μ mPG) as (memG) "[Hmem Rmem]".
-      iModIntro.
-      iExists (fun σ _ => regs_inv (H := (SailRegGS _ spec_name)) (σ.1) ∗ mem_inv memG (σ.2))%I.
-      iExists _.
-      iSplitR "Hs2 Rmem".
-      * iSplitL "Hs1".
-        + iExists (RegStore_to_map γ).
-          by iFrame.
-        + iFrame.
-      * iPoseProof (trips sailΣ (SailGS Hinv (SailRegGS reg_pre_inG spec_name) memG) with "[Rmem Hs2]") as "trips'".
-        + iFrame.
-          unfold RegStore_to_map.
-          iApply (own_RegStore_to_map_reg_pointsTos (H := SailRegGS reg_pre_inG spec_name)(γ := γ) (l := finite.enum (sigT 𝑹𝑬𝑮)) with "Hs2").
-          eapply finite.NoDup_enum.
-        + iApply (wp_mono with "trips'").
-          by iIntros ([δ3 v]).
-  Qed.
-End Adequacy.
-End IrisSignatureRules.
-
-Module Type IrisInstance (B : Base) (PROG : Program B) (SEM : Semantics B PROG) (SIG : Signature B) (IB : IrisBase B PROG SEM) :=
-  IrisPredicates B PROG SEM SIG IB <+ IrisSignatureRules B PROG SEM SIG IB.
-
-(*
- * The following module defines the parts of the Iris model that must depend on the Specification, not just on the Signature.
- * This is kept to a minimum (see comment for the IrisInstance module).
- *)
-Module IrisInstanceWithContracts
-  (Import B     : Base)
-  (Import PROG  : Program B)
-  (Import SEM   : Semantics B PROG)
-  (Import SIG   : Signature B)
-  (Import SPEC  : Specification B PROG SIG)
-  (Import IB    : IrisBase B PROG SEM)
-  (Import II    : IrisInstance B PROG SEM SIG IB)
-  (Import PLOG  : ProgramLogicOn B PROG SIG SPEC).
-
-  Section WithSailGS.
-  Import ProgramLogic.
-  Context {Σ} {sG : sailGS Σ}.
-
-  Definition ValidContractEnvSem (cenv : SepContractEnv) : iProp Σ :=
-    (∀ σs σ (f : 𝑭 σs σ),
-      match cenv σs σ f with
-      | Some c => ValidContractSem (FunDef f) c
-      | None => True
-      end)%I.
-
-  Definition ForeignSem :=
-    ∀ (Γ : PCtx) (τ : Ty)
-      (Δ : PCtx) f (es : NamedEnv (Exp Γ) Δ) (δ : CStore Γ),
-      match CEnvEx f with
-      | MkSepContract _ _ Σ' θΔ req result ens =>
-        forall (ι : Valuation Σ'),
-        evals es δ = inst θΔ ι ->
-        ⊢ semTriple δ (interpret_assertion req ι) (stm_foreign f es)
-          (fun v δ' => interpret_assertion ens (env.snoc ι (result∷τ) v) ∗ bi_pure (δ' = δ))
-      end.
-
-  Definition LemmaSem : Prop :=
-    forall (Δ : PCtx) (l : 𝑳 Δ),
-      ValidLemma (LEnv l).
-
-  Lemma iris_rule_stm_call_forwards {Γ} (δ : CStore Γ)
-        {Δ σ} (f : 𝑭 Δ σ) (c : SepContract Δ σ) (es : NamedEnv (Exp Γ) Δ)
-        (P : iProp Σ)
-        (Q : Val σ -> iProp Σ) :
-        CEnv f = Some c ->
-        CTriple (evals es δ) P Q c ->
-        (⊢ ▷ ValidContractEnvSem CEnv -∗
-           semTriple δ P (stm_call f es) (fun v δ' => Q v ∧ bi_pure (δ = δ')))%I.
-  Proof.
-    iIntros (ceq ctrip) "cenv P".
-    rewrite wp_unfold. cbn.
-    iIntros ([regs μ] ns ks1 ks nt) "Hregs".
-    iMod (fupd_mask_subseteq empty) as "Hclose"; first set_solver.
-    iModIntro.
-    iSplitR; [trivial|].
-    iIntros (e2 [regs2 μ2] efs) "%".
-    dependent elimination H.
-    dependent elimination s.
-    iModIntro. iModIntro. iModIntro.
-    iMod "Hclose" as "_".
-    iModIntro.
-    iFrame.
-    iSplitL; [|trivial].
-    destruct ctrip.
-    cbv [lentails lex land lprop lsep lall lwand IProp] in H.
-    iPoseProof (H with "P") as (ι Heq) "[req consr]". clear H.
-    iApply wp_compat_call_frame. rewrite Heq.
-    iSpecialize ("cenv" $! _ _ f0).
-    rewrite ceq.
-    iPoseProof ("cenv" $! ι with "req") as "wpf0".
-    iApply (wp_frame_wand with "consr").
-    iApply (wp_mono with "wpf0").
-    intros [v δ3]; cbn.
-    iIntros "ens consr".
-    iSplitL; [|trivial].
-    by iApply "consr".
-  Qed.
-
-  Lemma iris_rule_stm_call_frame {Γ} (δ : CStore Γ)
-        (Δ : PCtx) (δΔ : CStore Δ) (τ : Ty) (s : Stm Δ τ)
-        (P : iProp Σ) (Q : Val τ -> CStore Γ -> iProp Σ) :
-        ⊢ (semTriple δΔ P s (fun v _ => Q v δ) -∗
-           semTriple δ P (stm_call_frame δΔ s) Q)%I.
-  Proof.
-    iIntros "trips P".
-    iSpecialize ("trips" with "P").
-    by iApply wp_compat_call_frame.
-  Qed.
-
-  Lemma iris_rule_stm_foreign
-    {Γ} (δ : CStore Γ) {τ} {Δ} (f : 𝑭𝑿 Δ τ) (es : NamedEnv (Exp Γ) Δ)
-    (P : iProp Σ) (Q : Val τ -> CStore Γ -> iProp Σ) :
-    ForeignSem ->
-    CTriple (evals es δ) P (λ v : Val τ, Q v δ) (CEnvEx f) ->
-    ⊢ semTriple δ P (stm_foreign f es) Q.
-  Proof.
-    iIntros (extSem ctrip).
-    specialize (extSem _ _ _ f es δ).
-    revert ctrip extSem.
-    generalize (CEnvEx f) as contractF.
-    intros contractF ctrip extSem.
-    destruct ctrip; cbn in extSem.
-    iIntros "P".
-    cbv [lentails lex land lprop lsep lall lwand IProp] in H.
-    iPoseProof (H with "P") as (ι Heq) "[req consr]". clear H.
-    iPoseProof (extSem ι Heq with "req") as "wpf".
-    iApply (wp_frame_wand with "consr").
-    iApply (wp_mono with "wpf").
-    intros [v δ3]; cbn.
-    iIntros "[ens %] consr". subst.
-    by iApply "consr".
-  Qed.
-
-  Lemma iris_rule_stm_lemmak
-    {Γ} (δ : CStore Γ) {τ} {Δ} (l : 𝑳 Δ) (es : NamedEnv (Exp Γ) Δ) (k : Stm Γ τ)
-    (P Q : iProp Σ) (R : Val τ -> CStore Γ -> iProp Σ) :
-    LemmaSem ->
-    LTriple (evals es δ) P Q (LEnv l) ->
-    ⊢ semTriple δ Q k R -∗
-      semTriple δ P (stm_lemmak l es k) R.
-  Proof.
-    iIntros (lemSem ltrip).
-    specialize (lemSem _ l).
-    revert ltrip lemSem.
-    generalize (LEnv l) as contractL.
-    intros contractL ltrip lemSem.
-    iIntros "tripk P".
-    rewrite wp_unfold. cbn.
-    iIntros (σ ns ks1 ks nt) "Hregs".
-    iMod (fupd_mask_subseteq empty) as "Hclose"; first set_solver.
-    iModIntro. iSplitR; [trivial|].
-    iIntros (e3 σ2 efs) "%".
-    dependent elimination H.
-    dependent elimination s.
-    iModIntro. iModIntro. iModIntro.
-    iMod "Hclose" as "_".
-    iModIntro; iFrame.
-    iSplitL; [|trivial].
-    iApply "tripk".
-    dependent elimination ltrip; cbn in lemSem.
-    iPoseProof (l with "P") as (ι Heq) "[req consr]". clear l.
-    iApply "consr".
-    by iApply lemSem.
-  Qed.
-
-  Lemma sound_stm
-    {Γ} {τ} (s : Stm Γ τ) {δ : CStore Γ}:
-    forall (PRE : iProp Σ) (POST : Val τ -> CStore Γ -> iProp Σ),
-      ForeignSem ->
-      LemmaSem ->
-      ⦃ PRE ⦄ s ; δ ⦃ POST ⦄ ->
-      ⊢ (□ ▷ ValidContractEnvSem CEnv -∗
-          semTriple δ PRE s POST)%I.
-  Proof.
-    iIntros (PRE POST extSem lemSem triple) "#vcenv".
-    iInduction triple as [x|x|x|x|x|x|x|x|x|x|x|x|x|x|x|x|x|x|x|x|x|x|x|x|x|x|x|x|x|x|x] "trips".
-    - by iApply iris_rule_consequence.
-    - by iApply iris_rule_frame.
-    - by iApply iris_rule_pull.
-    - by iApply iris_rule_exist.
-    - iApply iris_rule_stm_val.
-      by iApply H.
-    - iApply iris_rule_stm_exp.
-      by iApply H.
-    - by iApply iris_rule_stm_let.
-    - by iApply iris_rule_stm_block.
-    - by iApply iris_rule_stm_if.
-    - by iApply iris_rule_stm_seq.
-    - by iApply iris_rule_stm_assertk.
-    - by iApply iris_rule_stm_fail.
-    - by iApply iris_rule_stm_match_list.
-    - by iApply iris_rule_stm_match_sum.
-    - by iApply iris_rule_stm_match_prod.
-    - by iApply iris_rule_stm_match_enum.
-    - by iApply iris_rule_stm_match_tuple.
-    - by iApply iris_rule_stm_match_union.
-    - by iApply iris_rule_stm_match_record.
-    - by iApply iris_rule_stm_match_bvec.
-    - by iApply iris_rule_stm_read_register.
-    - by iApply iris_rule_stm_write_register.
-    - by iApply iris_rule_stm_assign_backwards.
-    - by iApply iris_rule_stm_assign_forwards.
-    - by iApply iris_rule_stm_call_forwards.
-    - by iApply iris_rule_stm_call_inline.
-    - by iApply iris_rule_stm_call_frame.
-    - by iApply iris_rule_stm_foreign.
-    - by iApply iris_rule_stm_lemmak.
-    - by iApply iris_rule_stm_bind.
-    - by iApply iris_rule_stm_debugk.
-  Qed.
-
-  Lemma sound :
-    ForeignSem -> LemmaSem -> ValidContractCEnv ->
-    ⊢ ValidContractEnvSem CEnv.
-  Proof.
-    intros extSem lemSem vcenv.
-    iLöb as "IH".
-    iIntros (σs σ f).
-    specialize (vcenv σs σ f).
-    destruct (CEnv f) as [[]|];[|trivial].
-    specialize (vcenv _ eq_refl).
-    iIntros (ι).
-    iApply (sound_stm extSem lemSem); [|trivial].
-    apply (vcenv ι).
-  Qed.
-
-  End WithSailGS.
-End IrisInstanceWithContracts.
+  (Import IP   : IrisPrelims B PROG SEM).
+  Parameter memGpreS : gFunctors -> Set.
+  (* The memGS field will normally always be instantiated to a type class. We
+     inline this field, so that instances declared by the library, e.g. the
+     [sailGS_memGS] superclass instance below, will always be instances for the
+     user-provided class instead of the [memGS] alias. In your client code, you
+     should always refer to your typeclass and refrain from using the [memGS]
+     alias completely. *)
+  Parameter Inline memGS : gFunctors -> Set.
+  Parameter memΣ : gFunctors.
+  Parameter memΣ_GpreS : forall {Σ}, subG memΣ Σ -> memGpreS Σ.
+  Parameter mem_inv : forall {Σ}, memGS Σ -> Memory -> iProp Σ.
+  Parameter mem_res : forall {Σ}, memGS Σ -> Memory -> iProp Σ.
+
+    (* Definition mem_inv `{sailG Σ} (μ : Z -> option Z) : iProp Σ := *)
+    (*   (∃ memmap, gen_heap_ctx memmap ∗ *)
+    (*      ⌜ map_Forall (fun (a : Z) v => μ a = Some v) memmap ⌝ *)
+    (*   )%I. *)
+
+  Parameter mem_inv_init : forall Σ (μ : Memory), memGpreS Σ ->
+                                         ⊢ |==> ∃ mG : memGS Σ, (mem_inv mG μ ∗ mem_res mG μ)%I.
+End IrisParameters.
+
+Module Type IrisResources
+  (Import B    : Base)
+  (Import PROG : Program B)
+  (Import SEM  : Semantics B PROG)
+  (Import IPre : IrisPrelims B PROG SEM)
+  (Import IP   : IrisParameters B PROG SEM IPre).
+  Class sailGpreS Σ := SailGpreS { (* resources for the implementation side *)
+                       sailGpresS_invGpreS : invGpreS Σ; (* for fancy updates, invariants... *)
+
+                       (* ghost variable for tracking state of registers *)
+                       reg_pre_inG : inG Σ regUR;
+
+                       (* ghost variable for tracking state of memory cells *)
+                       sailPreG_gen_memGpreS : memGpreS Σ
+                     }.
+  #[export] Existing Instance sailGpresS_invGpreS.
+  #[export] Existing Instance reg_pre_inG.
+  Class sailGS Σ := SailGS { (* resources for the implementation side *)
+                       sailGS_invGS : invGS Σ; (* for fancy updates, invariants... *)
+                       sailGS_sailRegGS : sailRegGS Σ;
+
+                       (* ghost variable for tracking state of memory cells *)
+                       sailGS_memGS : memGS Σ
+                     }.
+  #[export] Existing Instance sailGS_invGS.
+  #[export] Existing Instance sailGS_sailRegGS.
+
+  (* We declare the memGS field as a class so that we can define the
+     [sailGS_memGS] field as an instance as well. Currently, the [Existing
+     Class] command does not support specifying a locality
+     (local/export/global), so it is not clear what the scope of this command
+     is. Because [memGS] will be inline on module functor applications, the
+     [sailGS_memGS] instance will refer to the user-provided class instead of
+     the [memGS] field. *)
+  Existing Class memGS.
+  #[export] Existing Instance sailGS_memGS.
+
+  #[export] Instance sailGS_irisGS {Γ τ} `{sailGS Σ} : irisGS (microsail_lang Γ τ) Σ := {
+    iris_invGS := sailGS_invGS;
+    state_interp σ ns κs nt := (regs_inv σ.1 ∗ mem_inv sailGS_memGS σ.2)%I;
+    fork_post _ := True%I; (* no threads forked in sail, so this is fine *)
+    num_laters_per_step _ := 0;
+    state_interp_mono _ _ _ _ := fupd_intro _ _;
+                                                                                }.
+  Global Opaque iris_invGS.
+End IrisResources.
+
+Module Type IrisBase (B : Base) (PROG : Program B) (SEM : Semantics B PROG) :=
+  IrisPrelims B PROG SEM <+ IrisParameters B PROG SEM <+ IrisResources B PROG SEM.
